Trying to stub out header equivalence.

deps/coq-poulet4/examples/BabyIPGrammarRel.v
@@ -8,13 +8,12 @@ Require Import P4String.
 Require Import Environment.
 Require Import Petr4.Monads.Monad.
 Require Import Coq.Lists.List.
+Require Import Coq.Strings.String.
+
 Import ListNotations.
+
 Open Scope nat_scope.
 Open Scope monad_scope.
-
-
-
-Compute foo.
 
 Definition eval_parser' pkt parser :=
   match parser with
@@ -37,7 +36,7 @@ Definition eval_parser' pkt parser :=
 Definition eval_parser pkt parser : option (Value * list bool) :=
   match eval_parser' pkt parser with
   | Some (inl _, env) =>
-    let get_pkt_and_hdr := 
+    let get_pkt_and_hdr :=
         let* pkt_val := env_str_lookup Info (MkP4String "packet") in
         let* hdr_val := env_str_lookup Info (MkP4String "hdr") in
         mret (hdr_val, pkt_val)
@@ -54,11 +53,107 @@ Definition eval_parser pkt parser : option (Value * list bool) :=
 Inductive header_repr: @Value Info -> Headers -> Prop :=
 .
 
+Fixpoint assoc_get {A: Type} (map: list (P4String * A)) (key: P4String) : option A :=
+  match map with
+  | nil => None
+  | (k, v) :: map' =>
+    if eqb k.(str) key.(str) then Some v else assoc_get map' key
+  end
+.
+
+Inductive bits_pos_equiv : positive -> {n: nat & bits n} -> Prop :=
+| bits_pos_equiv_base: bits_pos_equiv xH (existT bits 1 (true, tt))
+(* TODO: Sensible way to implement this comparison; note that bits are given msb to lsb *)
+.
+
+Inductive bits_Z_equiv : Z -> {n: nat & bits n} -> Prop :=
+| bits_Z_equiv_zero : forall n, bits_Z_equiv Z0 (existT bits n zero_bits)
+(* TODO: A way to make the stuff below typecheck. *)
+(* | bits_Z_equiv_pos: forall n p b, bits_pos_equiv p b -> bits_Z_equiv (Zpos p) (existT bits (S n) (false, projT2 b)) *)
+.
+
+Definition bits_equiv_header (val: list (P4String * @ValueBase Info)) (key: string) (n: nat) (other: option (bits n)) :=
+  match assoc_get val (MkP4String key), other with
+  | Some (ValBaseBit n' b), Some other' =>
+    n = n' /\ bits_Z_equiv b (existT bits n other')
+  | _, _ => False
+  end
+.
+
+Definition ip_header_equiv (val: @ValueBase Info) (hdrs: IPHeader) : Prop :=
+  match val with
+  | ValBaseHeader val' true =>
+    bits_equiv_header val' "src" 8 hdrs.(src) /\
+    bits_equiv_header val' "dst" 8 hdrs.(dest) /\
+    bits_equiv_header val' "proto" 4 hdrs.(proto)
+  | _ => False
+  end
+.
+
+Definition tcp_header_equiv (val: @ValueBase Info) (hdrs: TCP) : Prop :=
+  match val with
+  | ValBaseHeader val' true =>
+    bits_equiv_header val' "sport" 8 hdrs.(sport_t) /\
+    bits_equiv_header val' "dport" 8 hdrs.(dport_t) /\
+    bits_equiv_header val' "flags" 4 hdrs.(flags_t) /\
+    bits_equiv_header val' "seq" 8 hdrs.(SimpleIPv4Monadic.seq)
+  | _ => False
+  end
+.
+
+Definition udp_header_equiv (val: @ValueBase Info) (hdrs: UDP) : Prop :=
+  match val with
+  | ValBaseHeader val' true =>
+    bits_equiv_header val' "sport" 8 hdrs.(sport_u) /\
+    bits_equiv_header val' "dport" 8 hdrs.(dport_u) /\
+    bits_equiv_header val' "flags" 4 hdrs.(flags_u)
+  | _ => False
+  end
+.
+
+Definition t_or_u_header_equiv (val: @ValueBase Info) (hdrs: TCP + UDP) : Prop :=
+  match val with
+  | ValBaseHeader val' true =>
+    match hdrs with
+    | inl tcp_hdrs =>
+      assoc_get val' (MkP4String "udp") = None /\
+      match assoc_get val' (MkP4String "tcp") with
+      | Some val'' =>
+        tcp_header_equiv val'' tcp_hdrs
+      | None => False
+      end
+    | inr udp_hdrs =>
+      assoc_get val' (MkP4String "tcp") = None /\
+      match assoc_get val' (MkP4String "udp") with
+      | Some val'' =>
+        udp_header_equiv val'' udp_hdrs
+      | None => False
+      end
+    end
+  | _ => False
+  end
+.
+
+Definition header_equiv (val: @Value Info) (hdrs: Headers) : Prop :=
+  match val with
+  | ValBase (ValBaseHeader val' true) =>
+    match assoc_get val' (MkP4String "ip") with
+    | Some ip_val => ip_header_equiv ip_val hdrs.(ip)
+    | None => False
+    end /\
+    match assoc_get val' (MkP4String "t_or_u") with
+    | Some t_or_u_val => t_or_u_header_equiv t_or_u_val hdrs.(transport)
+    | None => False
+    end
+  | _ => False
+  end
+.
+
 Theorem parser_grammar_sound :
   forall p p' hdr hdr_rec parser_state,
     eval_parser p MyParser = Some (hdr, p') ->
     State.run_with_state (init_state p) Headers_p = (inl hdr_rec, parser_state) ->
-    header_repr hdr hdr_rec /\
+    header_equiv hdr hdr_rec /\
     p' = parser_state.(pkt).
 Proof.
   intros.
